Simple_Networks/Generalized_Network_Language_Model_Checking.thy
@@ -1,0 +1,1493 @@
+theory Generalized_Network_Language_Model_Checking
+  imports TA_Library.Temporal_Logics Generalized_Network_Language_Impl_Refine
+    Uppaal_Networks.UPPAAL_Model_Checking TA_Library.Abstract_Term
+begin
+
+section \<open>Product Bisimulation\<close>
+
+no_notation State_Networks.step_sn ("_ \<turnstile> \<langle>_, _, _\<rangle> \<rightarrow>\<^bsub>_\<^esub> \<langle>_, _, _\<rangle>" [61,61,61,61,61] 61)
+
+text \<open>
+  We have proved the necessary theorems already but we need to lift it to
+  the case where delay and action transitions are strictly alternating.
+\<close>
+inductive step_u' ::
+  "('a, 's, 'c, 't :: time, 'x, 'v :: linorder) nta \<Rightarrow> 's list \<Rightarrow> ('x \<rightharpoonup> 'v) \<Rightarrow> ('c, 't) cval
+  \<Rightarrow> 's list \<Rightarrow> ('x \<rightharpoonup> 'v) \<Rightarrow> ('c, 't) cval \<Rightarrow> bool"
+("_ \<turnstile> \<langle>_, _, _\<rangle> \<rightarrow> \<langle>_, _, _\<rangle>" [61,61,61,61] 61) where
+  "A \<turnstile> \<langle>L, s, u\<rangle> \<rightarrow> \<langle>L'', s'', u''\<rangle>" if
+  "A \<turnstile> \<langle>L, s, u\<rangle> \<rightarrow>\<^bsub>Del\<^esub> \<langle>L', s', u'\<rangle>"
+  "a \<noteq> Del"
+  "A \<turnstile> \<langle>L', s', u'\<rangle> \<rightarrow>\<^bsub>a\<^esub> \<langle>L'', s'', u''\<rangle>"
+
+inductive_cases step'_elims: "A \<turnstile>' \<langle>(L, s), u\<rangle> \<rightarrow> \<langle>(L', s'), u'\<rangle>"
+
+inductive_cases step_u'_elims: "A \<turnstile> \<langle>L, s, u\<rangle> \<rightarrow> \<langle>L', s', u'\<rangle>"
+
+theorem Bisimulation_Invariant_strong_intro:
+  fixes A :: "'a \<Rightarrow> 'a \<Rightarrow> bool"
+    and P :: "'a \<Rightarrow> bool"
+    and B :: "'a \<Rightarrow> 'a \<Rightarrow> bool"
+  assumes "\<And>a b. A a b \<Longrightarrow> P a \<Longrightarrow> B a b"
+    and "\<And>a b. B a b \<Longrightarrow> P a \<Longrightarrow> A a b"
+    and "\<And>a b. P a \<Longrightarrow> A a b \<Longrightarrow> P b"
+  shows "Bisimulation_Invariant A B (=) P P"
+  apply standard
+  subgoal A for a b a'
+    by (blast intro: assms)
+  subgoal B for a b a'
+    by (blast intro: assms)
+  subgoal C for a b
+    by (rule assms)
+  subgoal D for a b
+    by (rule C, assumption) (rule assms)
+  done
+
+context Prod_TA_Defs
+begin
+
+definition
+  "all_prop L s = (L \<in> states \<and> bounded bounds s)"
+
+lemma all_prop_boundedD[dest]:
+  "bounded bounds s" if "all_prop L s"
+  using that unfolding all_prop_def ..
+
+lemma all_prop_statesD[dest]:
+  "L \<in> states" if "all_prop L s"
+  using that unfolding all_prop_def ..
+
+end (* Prod TA Defs *)
+
+
+context Prod_TA
+begin
+
+lemma prod_action_step_not_eq_delay:
+  "a \<noteq> Del" if "prod_ta \<turnstile> \<langle>(L, s), u\<rangle> \<rightarrow>\<^bsub>a\<^esub> \<langle>(L', s'), u'\<rangle>"
+  using that
+  by cases (auto simp: trans_of_def prod_ta_def trans_prod_def trans_int_def trans_sync_def)
+
+end
+
+locale Prod_TA_urge =
+  Prod_TA + assumes urgency_removed: "\<forall>N \<in> set (fst (snd A)). urgent N = {}"
+begin
+
+lemma prod_all_prop_inv:
+  "all_prop L' s'" if "all_prop L s" "prod_ta \<turnstile> \<langle>(L, s), u\<rangle> \<rightarrow> \<langle>(L', s'), u'\<rangle>"
+  using that unfolding all_prop_def
+  by (auto elim: bounded_inv states_inv simp: step_iff[symmetric, OF _ _ urgency_removed])
+
+lemma prod_all_prop_inv':
+  "all_prop L' s'" if "all_prop L s" "prod_ta \<turnstile>' \<langle>(L, s), u\<rangle> \<rightarrow> \<langle>(L', s'), u'\<rangle>"
+  using that by (auto intro: prod_all_prop_inv elim!: step'_elims)
+
+interpretation prod_bisim:
+  Bisimulation_Invariant
+  "(\<lambda> (L, s, u) (L', s', u'). prod_ta \<turnstile>' \<langle>(L, s), u\<rangle> \<rightarrow> \<langle>(L', s'), u'\<rangle>)"
+  "(\<lambda> (L, s, u) (L', s', u'). A \<turnstile> \<langle>L, s, u\<rangle> \<rightarrow> \<langle>L', s', u'\<rangle>)"
+  "(=)"
+  "(\<lambda> (L, s, u). all_prop L s)"
+  "(\<lambda> (L, s, u). all_prop L s)"
+  apply (rule Bisimulation_Invariant_strong_intro; clarsimp)
+  subgoal
+    by (auto intro: step_u'.intros simp: all_prop_def
+             dest: action_sound prod_action_step_not_eq_delay delay_sound[OF _ _ _ urgency_removed]
+             elim!: step'_elims)
+  subgoal
+    by (auto 4 4 dest: prod_all_prop_inv action_complete elim: delay_complete elim!: step_u'_elims)
+  subgoal
+    by (rule prod_all_prop_inv')
+  done
+
+lemmas prod_bisim_intro = prod_bisim.Bisimulation_Invariant_axioms
+
+end (* Prod TA *)
+
+
+section \<open>The final semantics\<close>
+
+text \<open>State formulas\<close>
+datatype ('n, 's, 'a, 'b) sexp =
+  true |
+  \<comment> \<open>Boolean connectives\<close>
+  not "('n, 's, 'a, 'b) sexp" | "and" "('n, 's, 'a, 'b) sexp" "('n, 's, 'a, 'b) sexp" |
+  or "('n, 's, 'a, 'b) sexp" "('n, 's, 'a, 'b) sexp" | imply "('n, 's, 'a, 'b) sexp" "('n, 's, 'a, 'b) sexp" |
+  \<comment> \<open>Does var \<open>a\<close> equal \<open>x\<close>?\<close>
+  eq 'a 'b |
+  le 'a 'b |
+  lt 'a 'b |
+  ge 'a 'b |
+  gt 'a 'b |
+  \<comment> \<open>Is procces \<open>i\<close> in location \<open>l\<close>?\<close>
+  loc 'n 's
+
+datatype ('n, 's, 'a, 'b) formula =
+  EX "('n, 's, 'a, 'b) sexp" | EG "('n, 's, 'a, 'b) sexp"
+| AX "('n, 's, 'a, 'b) sexp" | AG "('n, 's, 'a, 'b) sexp"
+| Leadsto "('n, 's, 'a, 'b) sexp" "('n, 's, 'a, 'b) sexp"
+
+fun check_sexp :: "(nat, 's, 'a, 'b :: linorder) sexp \<Rightarrow> 's list \<Rightarrow> ('a \<Rightarrow> 'b) \<Rightarrow> bool" where
+  "check_sexp sexp.true _ _ \<longleftrightarrow> True" |
+  "check_sexp (not e) L s \<longleftrightarrow> \<not> check_sexp e L s" |
+  "check_sexp (and e1 e2) L s \<longleftrightarrow> check_sexp e1 L s \<and> check_sexp e2 L s" |
+  "check_sexp (sexp.or e1 e2) L s \<longleftrightarrow> check_sexp e1 L s \<or> check_sexp e2 L s" |
+  "check_sexp (imply e1 e2) L s \<longleftrightarrow> check_sexp e1 L s \<longrightarrow> check_sexp e2 L s" |
+  "check_sexp (eq i x) L s \<longleftrightarrow> s i = x" |
+  "check_sexp (le i x) L s \<longleftrightarrow> s i \<le> x" |
+  "check_sexp (lt i x) L s \<longleftrightarrow> s i < x" |
+  "check_sexp (ge i x) L s \<longleftrightarrow> s i \<ge> x" |
+  "check_sexp (gt i x) L s \<longleftrightarrow> s i > x" |
+  "check_sexp (loc i x) L s \<longleftrightarrow> L ! i = x"
+
+fun locs_of_sexp :: "('n, 's, 'a, 'b) sexp \<Rightarrow> 'n set" where
+  "locs_of_sexp (not e) = locs_of_sexp e" |
+  "locs_of_sexp (and e1 e2) = locs_of_sexp e1 \<union> locs_of_sexp e2" |
+  "locs_of_sexp (sexp.or e1 e2) = locs_of_sexp e1 \<union> locs_of_sexp e2" |
+  "locs_of_sexp (imply e1 e2) = locs_of_sexp e1 \<union> locs_of_sexp e2" |
+  "locs_of_sexp (loc i x) = {i}" |
+  "locs_of_sexp _ = {}"
+
+fun vars_of_sexp :: "('n, 's, 'a, 'b) sexp \<Rightarrow> 'a set" where
+  "vars_of_sexp (not e) = vars_of_sexp e" |
+  "vars_of_sexp (and e1 e2) = vars_of_sexp e1 \<union> vars_of_sexp e2" |
+  "vars_of_sexp (sexp.or e1 e2) = vars_of_sexp e1 \<union> vars_of_sexp e2" |
+  "vars_of_sexp (imply e1 e2) = vars_of_sexp e1 \<union> vars_of_sexp e2" |
+  "vars_of_sexp (eq i x) = {i}" |
+  "vars_of_sexp (lt i x) = {i}" |
+  "vars_of_sexp (le i x) = {i}" |
+  "vars_of_sexp (ge i x) = {i}" |
+  "vars_of_sexp (gt i x) = {i}" |
+  "vars_of_sexp _ = {}"
+
+fun locs_of_formula :: "('n, 's, 'a, 'b) formula \<Rightarrow> 'n set" where
+  "locs_of_formula (formula.EX \<phi>) = locs_of_sexp \<phi>" |
+  "locs_of_formula (EG \<phi>) = locs_of_sexp \<phi>" |
+  "locs_of_formula (AX \<phi>) = locs_of_sexp \<phi>" |
+  "locs_of_formula (AG \<phi>) = locs_of_sexp \<phi>" |
+  "locs_of_formula (Leadsto \<phi> \<psi>) = locs_of_sexp \<phi> \<union> locs_of_sexp \<psi>"
+
+fun vars_of_formula :: "('n, 's, 'a, 'b) formula \<Rightarrow> 'a set" where
+  "vars_of_formula (formula.EX \<phi>) = vars_of_sexp \<phi>" |
+  "vars_of_formula (EG \<phi>) = vars_of_sexp \<phi>" |
+  "vars_of_formula (AX \<phi>) = vars_of_sexp \<phi>" |
+  "vars_of_formula (AG \<phi>) = vars_of_sexp \<phi>" |
+  "vars_of_formula (Leadsto \<phi> \<psi>) = vars_of_sexp \<phi> \<union> vars_of_sexp \<psi>"
+
+fun hd_of_formula :: "(nat, 's, 'a, 'b) formula \<Rightarrow> 's list \<Rightarrow> ('a \<Rightarrow> 'b :: linorder) \<Rightarrow> bool" where
+  "hd_of_formula (formula.EX \<phi>) L s = check_sexp \<phi> L s" |
+  "hd_of_formula (EG \<phi>) L s = check_sexp \<phi> L s" |
+  "hd_of_formula (AX \<phi>) L s = Not (check_sexp \<phi> L s)" |
+  "hd_of_formula (AG \<phi>) L s = Not (check_sexp \<phi> L s)" |
+  "hd_of_formula (Leadsto \<phi> _) L s = check_sexp \<phi> L s"
+
+definition models ("_,_ \<Turnstile> _" [61,61] 61) where
+  "A,a\<^sub>0 \<Turnstile> \<Phi> \<equiv> (case \<Phi> of
+    formula.EX \<phi> \<Rightarrow>
+      Graph_Defs.Ex_ev
+        (\<lambda> (L, s, u) (L', s', u'). A \<turnstile> \<langle>L, s, u\<rangle> \<rightarrow> \<langle>L', s', u'\<rangle>)
+        (\<lambda> (L, s, _). check_sexp \<phi> L (the o s))
+  | formula.EG \<phi> \<Rightarrow>
+      Graph_Defs.Ex_alw
+        (\<lambda> (L, s, u) (L', s', u'). A \<turnstile> \<langle>L, s, u\<rangle> \<rightarrow> \<langle>L', s', u'\<rangle>)
+        (\<lambda> (L, s, _). check_sexp \<phi> L (the o s))
+  | formula.AX \<phi> \<Rightarrow>
+      Graph_Defs.Alw_ev
+        (\<lambda> (L, s, u) (L', s', u'). A \<turnstile> \<langle>L, s, u\<rangle> \<rightarrow> \<langle>L', s', u'\<rangle>)
+        (\<lambda> (L, s, _). check_sexp \<phi> L (the o s))
+  | formula.AG \<phi> \<Rightarrow>
+      Graph_Defs.Alw_alw
+        (\<lambda> (L, s, u) (L', s', u'). A \<turnstile> \<langle>L, s, u\<rangle> \<rightarrow> \<langle>L', s', u'\<rangle>)
+        (\<lambda> (L, s, _). check_sexp \<phi> L (the o s))
+  | formula.Leadsto \<phi> \<psi> \<Rightarrow>
+      Graph_Defs.leadsto
+        (\<lambda> (L, s, u) (L', s', u'). A \<turnstile> \<langle>L, s, u\<rangle> \<rightarrow> \<langle>L', s', u'\<rangle>)
+        (\<lambda> (L, s, _). check_sexp \<phi> L (the o s))
+        (\<lambda> (L, s, _). check_sexp \<psi> L (the o s))
+  ) a\<^sub>0"
+
+lemmas models_iff = models_def[unfolded Graph_Defs.Ex_alw_iff Graph_Defs.Alw_alw_iff]
+
+definition prop_of where
+  "prop_of \<phi> = PropC (\<lambda>(L, s, _). check_sexp \<phi> L (the o s))"
+
+fun ctl_of where
+  "ctl_of (formula.EX \<phi>) = ctl_formula.EX (prop_of \<phi>)"
+| "ctl_of (formula.EG \<phi>) = ctl_formula.EG (prop_of \<phi>)"
+| "ctl_of (formula.AX \<phi>) = ctl_formula.AX (prop_of \<phi>)"
+| "ctl_of (formula.AG \<phi>) = ctl_formula.AG (prop_of \<phi>)"
+| "ctl_of (formula.Leadsto \<phi> \<psi>) =
+  ctl_formula.AG (ctl_formula.ImpliesC (prop_of \<phi>) (ctl_formula.AX (prop_of \<psi>)))"
+
+context
+  fixes A :: "('a, 's, 'c, 't :: time, 'x, 'v :: linorder) nta"
+begin
+
+interpretation Graph_Defs "\<lambda> (L, s, u) (L', s', u'). A \<turnstile> \<langle>L, s, u\<rangle> \<rightarrow> \<langle>L', s', u'\<rangle>" .
+
+lemma models_ctl_iff:
+  "A,a\<^sub>0 \<Turnstile> \<Phi> \<longleftrightarrow> models_ctl (ctl_of \<Phi>) a\<^sub>0"
+  by (cases \<Phi>) (simp_all add: models_def prop_of_def leadsto_def)
+
+end
+
+fun check_sexpi :: "(nat, 's, nat, int) sexp \<Rightarrow> 's list \<Rightarrow> int list \<Rightarrow> bool" where
+  "check_sexpi sexp.true _ _ \<longleftrightarrow> True" |
+  "check_sexpi (not e) L s \<longleftrightarrow> \<not> check_sexpi e L s" |
+  "check_sexpi (and e1 e2) L s \<longleftrightarrow> check_sexpi e1 L s \<and> check_sexpi e2 L s" |
+  "check_sexpi (sexp.or e1 e2) L s \<longleftrightarrow> check_sexpi e1 L s \<or> check_sexpi e2 L s" |
+  "check_sexpi (imply e1 e2) L s \<longleftrightarrow> check_sexpi e1 L s \<longrightarrow> check_sexpi e2 L s" |
+  "check_sexpi (eq i x) L s \<longleftrightarrow> s ! i = x" |
+  "check_sexpi (le i x) L s \<longleftrightarrow> s ! i \<le> x" |
+  "check_sexpi (lt i x) L s \<longleftrightarrow> s ! i < x" |
+  "check_sexpi (ge i x) L s \<longleftrightarrow> s ! i \<ge> x" |
+  "check_sexpi (gt i x) L s \<longleftrightarrow> s ! i > x" |
+  "check_sexpi (loc i x) L s \<longleftrightarrow> L ! i = x"
+
+fun hd_of_formulai :: "(nat, 's, nat, int) formula \<Rightarrow> 's list \<Rightarrow> int list \<Rightarrow> bool" where
+  "hd_of_formulai (formula.EX \<phi>) L s = check_sexpi \<phi> L s" |
+  "hd_of_formulai (EG \<phi>) L s = check_sexpi \<phi> L s" |
+  "hd_of_formulai (AX \<phi>) L s = Not (check_sexpi \<phi> L s)" |
+  "hd_of_formulai (AG \<phi>) L s = Not (check_sexpi \<phi> L s)" |
+  "hd_of_formulai (Leadsto \<phi> _) L s = check_sexpi \<phi> L s"
+
+
+
+(* XXX Stop locale constant unfolding in simplifier *)
+lemma all_prop_weak_cong[cong]:
+  "Prod_TA_Defs.all_prop A = Prod_TA_Defs.all_prop A" for A
+  by(rule HOL.refl)
+lemma equiv'_weak_cong[cong]:
+  "Bisimulation_Invariant.equiv' R P Q = Bisimulation_Invariant.equiv' R P Q" for R P Q
+  by (rule HOL.refl)
+lemma equiv'_weak_cong2[cong]:
+  "Simulation_Invariant.equiv' R P Q = Simulation_Invariant.equiv' R P Q" for R P Q
+  by (rule HOL.refl)
+lemma models_ctl_weak_cong[cong]:
+  "Graph_Defs.models_ctl E = Graph_Defs.models_ctl E" for E
+  by (rule HOL.refl)
+lemma models_path_weak_cong[cong]:
+  "Graph_Defs.models_path E = Graph_Defs.models_path E" for E
+  by (rule HOL.refl)
+lemma models_state_weak_cong[cong]:
+  "Graph_Defs.models_state E = Graph_Defs.models_state E" for E
+  by (rule HOL.refl)
+lemma models_ltl_weak_cong[cong]:
+  "Graph_Defs.models_ltlc E = Graph_Defs.models_ltlc E" for E
+  by (rule HOL.refl)
+lemma models_weak_cong[cong]:
+  "models E = models E"
+  for E by (rule HOL.refl)
+
+
+
+
+section \<open>Instantiating the Model Checking Locale\<close>
+
+locale Generalized_Network_Impl_nat_urge =
+  Generalized_Network_Impl_nat + assumes no_urgency: "\<forall> (_, U, _, _) \<in> set automata. U = []"
+
+text \<open>
+  This locale certifies that a given local clock ceiling is correct.
+  Moreover, we certify that the vector of initial locations has outgoing transitions for
+  each automaton, and that all variables of the initial state are in bounds.
+\<close>
+locale Generalized_Network_Impl_nat_ceiling_start_state =
+  Generalized_Network_Impl_nat_urge +
+  fixes k :: "nat list list list"
+    and L\<^sub>0 :: "nat list"
+    and s\<^sub>0 :: "(nat \<times> int) list"
+    and formula :: "(nat, nat, nat, int) formula"
+    and show_clock :: "nat \<Rightarrow> string"
+    and show_state :: "nat list \<times> int list \<Rightarrow> string"
+  assumes k_ceiling:
+    "\<forall>i < n_ps. \<forall>(l, g) \<in> set ((snd o snd o snd) (automata ! i)).
+      \<forall>(x, m) \<in> collect_clock_pairs g. m \<le> int (k ! i ! l ! x)"
+    "\<forall>i < n_ps. \<forall>(l, _, g, _) \<in> set ((fst o snd o snd) (automata ! i)).
+      (\<forall>(x, m) \<in> collect_clock_pairs g. m \<le> int (k ! i ! l ! x))"
+  and k_resets:
+    "\<forall>i < n_ps. \<forall> (l, b, g, a, upd, r, l') \<in> set ((fst o snd o snd) (automata ! i)).
+       \<forall>c \<in> {0..<m+1} - set r. k ! i ! l' ! c \<le> k ! i ! l ! c"
+  and k_length:
+    "length k = n_ps" "\<forall> i < n_ps. length (k ! i) = num_states i"
+    "\<forall> xs \<in> set k. \<forall> xxs \<in> set xs. length xxs = m + 1"
+  and k_0:
+    "\<forall>i < n_ps. \<forall>l < num_states i. k ! i ! l ! 0 = 0"
+  and inv_unambiguous:
+    "\<forall>(_, _, _, inv) \<in> set automata. distinct (map fst inv)"
+  and s\<^sub>0_bounded: "bounded bounds (map_of s\<^sub>0)"
+  and L\<^sub>0_len: "length L\<^sub>0 = n_ps"
+  and L\<^sub>0_has_trans: "\<forall>i < n_ps. L\<^sub>0 ! i \<in> fst ` set ((fst o snd o snd) (automata ! i))"
+  and vars_of_formula: "vars_of_formula formula \<subseteq> {0..<n_vs}"
+  (* and num_states_length: "\<forall>i<n_ps. num_states i = length (fst (snd (automata ! i)))" *)
+begin
+
+text \<open>
+The ceiling \<open>k\<close> is correct for each individual automaton in the network.
+We now construct a ceiling for the product automaton:
+\<close>
+definition
+  "k_fun l c \<equiv>
+    if (c > 0 \<and> c \<le> m) \<and> fst l \<in> states then Max {k ! i ! (fst l ! i) ! c | i . i < n_ps} else 0"
+
+lemma (in -) default_map_of_distinct:
+  "(k, default_map_of x xs k) \<in> set xs \<union> {(k, x)}" if "distinct (map fst xs)"
+  unfolding default_map_of_alt_def by clarsimp (simp add: map_of_eq_Some_iff[OF that])
+
+lemma N_inv:
+  "(L ! i, inv (N i) (L ! i)) \<in> set ((snd o snd o snd) (automata ! i)) \<union> {(L ! i, [])}"
+  if "i < n_ps"
+  unfolding N_def comp_def fst_conv snd_conv inv_def
+  using that
+  apply (subst nth_map)
+   apply (simp add: n_ps_def; fail)
+  apply (clarsimp split: prod.split simp: automaton_of_def)
+  subgoal for _ _ _ xs
+    using default_map_of_distinct[of xs "L ! i" "[]"] inv_unambiguous that
+    by (auto dest!: nth_mem simp: n_ps_def)
+  done
+
+lemma (in -) subset_nat_0_atLeastLessThan_conv:
+  "S \<subseteq> {0..<n::nat} \<longleftrightarrow> (\<forall> x \<in> S. x < n)"
+  by auto
+
+lemma k_ceiling_rule:
+  "m \<le> int (k ! i ! l ! x)"
+  if "i < n_ps" "(l, b, g, xx) \<in> set ((fst o snd o snd) (automata ! i))"
+     "(x, m) \<in> collect_clock_pairs g"
+  for i l x g xx
+  using that k_ceiling(2) by fastforce
+
+lemma k_ceiling_1:
+  "\<forall>s. \<forall>L \<in> states. \<forall>(x,m) \<in> clkp_set prod_ta (L, s). m \<le> k_fun (L, s) x"
+proof safe
+  fix L s c x
+  assume \<open>L \<in> states\<close> \<open>(c, x) \<in> Closure.clkp_set prod_ta (L, s)\<close>
+  have "0 < c" "c \<le> m"
+  proof -
+    from \<open>(c, x) \<in> _\<close> have "(c, x) \<in> Timed_Automata.clkp_set prod_ta"
+      unfolding TA_clkp_set_unfold by auto
+    with clock_range show "0 < c" "c \<le> m"
+      by auto
+  qed
+  with \<open>L \<in> _\<close> have "k_fun (L, s) c = Max {k ! i ! (L ! i) ! c | i . i < n_ps}"
+    unfolding k_fun_def by auto
+  have Max_aux: "x \<le> int (Max {k ! i ! (L ! i) ! c |i. i < n_ps})"
+    if "x \<le> int (k ! p ! (L ! p) ! c)" "p < n_ps" for p
+  proof -
+    from \<open>p < n_ps \<close> have "k ! p ! (L ! p) ! c \<le> Max {k ! i ! (L ! i) ! c |i. i < n_ps}"
+      by (intro Max_ge) auto
+    with \<open>x \<le> _\<close> show ?thesis
+      by simp
+  qed
+  from \<open>(c, x) \<in> _\<close> show \<open>x \<le> k_fun (L, s) c\<close>
+    unfolding clkp_set_def
+  proof safe
+    assume \<open>(c, x) \<in> Closure.collect_clki (inv_of prod_ta) (L, s)\<close>
+    then show \<open>x \<le> k_fun (L, s) c\<close>
+      using k_ceiling(1) unfolding collect_clki_def \<open>k_fun (L, s) c = _\<close>
+      by (clarsimp simp add: prod_inv_def collect_clock_pairs_def k_fun_def)
+         (frule N_inv, rule Max_aux; fastforce)
+  next
+    assume \<open>(c, x) \<in> Closure.collect_clkt (trans_of prod_ta) (L, s)\<close>
+    then show \<open>x \<le> k_fun (L, s) c\<close>
+      unfolding collect_clkt_def \<open>k_fun (L, s) c = _\<close>
+      apply (clarsimp simp: trans_prod_def collect_clock_pairs_def k_fun_def)
+      apply safe
+      subgoal \<comment> \<open>trans_int\<close>
+        using k_ceiling(2) unfolding trans_int_def
+        apply (clarsimp simp: mem_trans_N_iff L_len subset_nat_0_atLeastLessThan_conv)
+        apply (fastforce intro!: Max_aux simp: collect_clock_pairs_def)
+        done
+      subgoal \<comment> \<open>trans_sync\<close>
+        using k_ceiling(2) unfolding trans_sync_tagged_def
+        by (clarsimp, tag- \<open>TRANS _\<close> \<open>SEL ''range''\<close>)
+           (fastforce intro!: Max_aux
+            simp: collect_clock_pairs_def mem_trans_N_iff L_len subset_nat_0_atLeastLessThan_conv)
+      done
+  qed
+qed
+
+lemma k_fun_mono':
+  "k_fun (L, s) c \<le> k_fun (L', s') c" if
+  "\<forall>i < n_ps. k ! i ! (L ! i) ! c \<le> k ! i ! (L' ! i) ! c" "L \<in> states" "L' \<in> states"
+  using that unfolding k_fun_def
+  apply clarsimp
+  apply (cases "n_ps = 0")
+   apply (simp; fail)
+  apply (rule Max.boundedI)
+    apply (simp; fail)
+   apply blast
+  apply safe
+  subgoal for _ i
+    by - (rule order.trans[where b = "k ! i ! (L' ! i) ! c"], auto intro: Max_ge)
+  done
+
+lemma k_fun_mono:
+  \<open>Max {k ! i ! (L ! i) ! c | i . i < n_ps} \<le> Max {k ! i ! (L' ! i) ! c | i . i < n_ps}\<close>
+  if \<open>\<forall>i < n_ps. k ! i ! (L ! i) ! c \<le> k ! i ! (L' ! i) ! c\<close>
+  apply (cases "n_ps = 0")
+   apply (simp; fail)
+  apply (rule Max.boundedI)
+    apply (simp; fail)
+   apply blast
+  apply safe
+  subgoal for _ i
+    using that by - (rule order.trans[where b = "k ! i ! (L' ! i) ! c"], auto intro: Max_ge)
+  done
+
+lemma (in -) fold_upds_aux1:
+  "fold (\<lambda>p L. L[p := g p]) ps xs ! i = xs ! i" if \<open>i \<notin> set ps\<close>
+  using that by (induction ps arbitrary: xs) auto
+
+lemma (in -) fold_upds_aux2:
+  "fold (\<lambda>p L. L[p := g p]) ps xs ! i = g i" if \<open>distinct ps\<close> \<open>i \<in> set ps\<close> \<open>i < length xs\<close>
+  using that by (induction ps arbitrary: xs) (auto simp: fold_upds_aux1)
+
+lemma (in -) fold_upds_aux_length:
+  "length (fold (\<lambda>p L. L[p := g p]) ps xs) = length xs"
+  by (induction ps arbitrary: xs) auto
+
+(* XXX Duplication *)
+lemma (in -) state_set_eq[simp]:
+  "Simulation_Graphs_TA.state_set A = state_set (trans_of A)"
+  unfolding Simulation_Graphs_TA.state_set_def state_set_def trans_of_def ..
+
+lemma prod_ta_step_statesD:
+  assumes "prod_ta \<turnstile> (L, s) \<longrightarrow>\<^bsup>g,a,r\<^esup> (L', s')"
+  shows "L \<in> states" "L' \<in> states"
+  using assms state_set_states by (fastforce dest: state_setI1 state_setI2)+
+
+lemma k_ceiling_2:
+  "\<forall>l g a r l'. \<forall> c \<le> m. prod_ta \<turnstile> l \<longrightarrow>\<^bsup>g,a,r\<^esup> l' \<and> c \<notin> set r \<longrightarrow> k_fun l' c \<le> k_fun l c"
+proof safe
+  fix L s g a r L' s' c
+  assume step: \<open>prod_ta \<turnstile> (L, s) \<longrightarrow>\<^bsup>g,a,r\<^esup> (L', s')\<close> and \<open>c \<le> m\<close> \<open>c \<notin> set r\<close>
+  from step have
+    \<open>Max {k ! i ! (L' ! i) ! c | i . i < n_ps} \<le> Max {k ! i ! (L ! i) ! c | i . i < n_ps}\<close>
+    apply simp
+    unfolding trans_prod_def
+    apply (clarsimp, erule disjE)
+    subgoal
+      using k_resets
+      unfolding trans_int_def
+      apply clarsimp
+      apply (rule k_fun_mono)
+      apply (clarsimp simp: mem_trans_N_iff L_len subset_nat_0_atLeastLessThan_conv)
+      subgoal for b f p aa l' i
+        using \<open>c \<le> m\<close> \<open>c \<notin> set r\<close> by (cases "p = i"; force simp add: L_len)
+      done
+    subgoal
+      unfolding trans_sync_tagged_def
+      apply simp
+      apply (rule k_fun_mono)
+      apply (clarsimp simp: )
+      subgoal premises [tagged] for sync bs gs as fs rs ls' ps i
+      proof -
+        have "distinct ps"
+          usingT \<open>SEL ''sublist''\<close> \<open>''sync''\<close> using action_set(3)
+          by (auto intro: subseq_distinct simp: syncs_def)
+        show ?thesis
+        proof (cases "i \<in> set ps")
+          case True
+          then have **: "fold (\<lambda>p L. L[p := ls' p]) ps L ! i = ls' i"
+            using \<open>distinct ps\<close> \<open>i < n_ps\<close> \<open>L \<in> states\<close> by (auto simp: fold_upds_aux2)
+          moreover have
+            "(L ! i, bs i, gs i, Com (as i), fs i, rs i, ls' i)
+            \<in> set (fst (snd (snd (automata ! i))))"
+            using True usingT \<open>TRANS _\<close> \<open>SEL ''range''\<close>
+            by (simp add: mem_trans_N_iff subset_nat_0_atLeastLessThan_conv)
+          moreover have "c\<in>{0..<Suc m} - set (rs i)"
+            using True \<open>c \<le> m\<close> \<open>c \<notin> set r\<close> \<open>r = _\<close> by fastforce
+          ultimately show ?thesis
+            using k_resets \<open>i < n_ps\<close> usingT \<open>''new loc''\<close> by (auto 4 3)
+        next
+          case False
+          then show ?thesis
+            usingT \<open>''new loc''\<close> by (simp add: fold_upds_aux1)
+        qed
+      qed
+      done
+    done
+  moreover from step have "L \<in> states" "L' \<in> states"
+    by - (rule prod_ta_step_statesD, assumption)+ 
+  ultimately show "k_fun (L', s') c \<le> k_fun (L, s) c"
+    using \<open>c \<le> m\<close> by (auto simp: k_fun_def)
+qed
+
+
+
+abbreviation F where "F \<equiv> \<lambda>(L, s). hd_of_formula formula L (the o s)"
+abbreviation "Fi \<equiv> \<lambda>(L, s). hd_of_formulai formula L s"
+
+lemma (in Generalized_Network_Impl_nat) check_sexp_check_sexpi:
+  "check_sexp e L (the o s) \<longleftrightarrow> check_sexpi e L s'"
+  if "state_rel s s'" "vars_of_sexp e \<subseteq> {0..<n_vs}"
+  using that unfolding state_rel_def by (induction e) auto
+
+lemma (in Generalized_Network_Impl_nat) hd_of_formula_hd_of_formulai:
+  "hd_of_formula \<phi> L (the o s) \<longleftrightarrow> hd_of_formulai \<phi> L s'"
+  if "state_rel s s'" "vars_of_formula \<phi> \<subseteq> {0..<n_vs}"
+  using that by (induction \<phi>) (auto simp: check_sexp_check_sexpi)
+
+lemma F_Fi:
+  "F l \<longleftrightarrow> Fi l'" if "(l', l) \<in> loc_rel"
+  using vars_of_formula that unfolding loc_rel_def by clarsimp (erule hd_of_formula_hd_of_formulai)
+
+
+abbreviation "l\<^sub>0 \<equiv> (L\<^sub>0, map_of s\<^sub>0)"
+abbreviation "s\<^sub>0i \<equiv> map (the o map_of s\<^sub>0) [0..<n_vs]"
+abbreviation "l\<^sub>0i \<equiv> (L\<^sub>0, s\<^sub>0i)"
+
+lemma state_rel_start:
+  "state_rel (map_of s\<^sub>0) s\<^sub>0i"
+  using s\<^sub>0_bounded unfolding state_rel_def bounded_def dom_bounds_eq by auto
+
+lemma statesI:
+  "L \<in> states" if "length L = n_ps" "\<forall>i<n_ps. L ! i \<in> fst ` set (fst (snd (snd (automata ! i))))"
+  using that unfolding states_def by (auto 4 3 simp: mem_trans_N_iff[symmetric])
+
+lemma L\<^sub>0_states[simp, intro]:
+  "L\<^sub>0 \<in> states"
+  using L\<^sub>0_has_trans L\<^sub>0_len by (auto intro: statesI)
+
+lemma l\<^sub>0_states'[simp, intro]:
+  "l\<^sub>0 \<in> states'"
+  using state_rel_start s\<^sub>0_bounded unfolding states'_def state_rel_def by auto
+
+print_locale Reachability_Problem_Defs
+
+sublocale reach: Reachability_Problem_Defs
+  prod_ta
+  l\<^sub>0
+  m
+  k_fun
+  F
+  .
+
+lemma (in -) collect_clkt_state_setI:
+  assumes "(x, d) \<in> Closure.collect_clkt (trans_of A) l"
+  shows "l \<in> state_set (trans_of A)" "l \<in> Simulation_Graphs_TA.state_set A"
+  using assms unfolding collect_clkt_def by (auto simp: state_set_def)
+
+lemma clkp_set_statesD:
+  fixes x d
+  assumes "(x, d)\<in>Closure.clkp_set prod_ta (L, s)"
+  shows "L \<in> states"
+  using assms
+  unfolding clkp_set_def collect_clki_def
+  apply safe
+  subgoal
+    apply simp
+    unfolding prod_inv_def
+    unfolding collect_clock_pairs_def
+    apply auto
+    done
+  apply (drule collect_clkt_state_setI)
+  using state_set_states by auto
+
+sublocale reach1: Reachability_Problem
+  prod_ta
+  l\<^sub>0
+  m
+  k_fun
+  F
+  apply standard
+  subgoal
+    apply safe
+    using k_ceiling_1
+    subgoal for L s x m
+      apply (cases "L \<in> states")
+       apply blast
+      apply (auto dest: clkp_set_statesD simp: k_fun_def)
+      done
+    done
+  subgoal
+    apply safe
+    subgoal for L s g a r L' s' c
+      apply (cases "c \<le> m")
+      using k_ceiling_2
+       apply force
+      apply (auto simp: k_fun_def)
+      done
+    done
+  subgoal
+    by (simp add: k_fun_def)
+  subgoal
+    by (simp add: k_fun_def)
+  done
+
+lemma states'_superset:
+  "{l\<^sub>0} \<union> Normalized_Zone_Semantics_Impl_Refine.state_set trans_prod \<subseteq> states'"
+  (is "{l\<^sub>0} \<union> ?S \<subseteq> states'")
+proof -
+  have "?S \<subseteq> states'"
+  proof clarsimp
+    fix L s
+    assume "(L, s) \<in> ?S"
+    then have "L \<in> states"
+      using state_set_states[unfolded trans_of_prod state_set_eq] by blast
+    moreover have "bounded bounds s"
+      using \<open>(L, s) \<in> _\<close>
+      unfolding state_set_def
+      unfolding trans_prod_def
+      unfolding trans_int_def trans_sync_def
+      by auto
+    ultimately show "(L, s) \<in> states'"
+      by (auto simp: states'_alt_def)
+  qed
+  then show ?thesis
+    by simp
+qed
+
+
+
+definition "k_i \<equiv> IArray (map (IArray o (map (IArray o map int))) k)"
+
+definition
+  "k_impl \<equiv> \<lambda>(l, _). IArray (map (\<lambda> c. Max {k_i !! i !! (l ! i) !! c | i. i < n_ps}) [0..<m+1])"
+
+(* XXX Duplication with UPPAAL_State_Networks_Impl_Refine *)
+lemma Max_int_commute:
+  "int (Max S) = Max (int ` S)" if "finite S" "S \<noteq> {}"
+  apply (rule mono_Max_commute)
+    apply rule
+  using that by auto
+
+lemma (in Generalized_Network_Impl_nat) n_ps_gt_0: "n_ps > 0"
+  using length_automata_eq_n_ps non_empty by auto
+
+lemma statesD:
+  "L ! i \<in> fst ` set (fst (snd (snd (automata ! i))))
+ \<or> L ! i \<in> (snd o snd o snd o snd o snd o snd) ` set (fst (snd (snd (automata ! i))))"
+  if "L \<in> states" "length L = n_ps" "i < n_ps"
+  using that unfolding states_def
+  apply auto
+  apply -
+  apply (elim allE impE, assumption)
+  apply auto
+   apply (force simp: mem_trans_N_iff)+
+  done
+
+lemma k_impl_k_fun:
+  "k_impl (L, s) = IArray (map (k_fun (L, s)) [0..<m+1])" if "L \<in> states"
+proof -
+  define k_i2 where "k_i2 i c = k_i !! i !! (L ! i) !! c" for i c
+  have k_i2_k: "k_i2 i c = k ! i ! (L ! i) ! c" if "i < n_ps" "c \<le> m" for i c
+  proof -
+    have "i < length k"
+      by (simp add: k_length(1) that(1))
+    moreover have "L ! i < length (k ! i)"
+      using L_i_len[OF _ \<open>L \<in> states\<close>] k_length(2) \<open>i < n_ps\<close> by auto
+    moreover have "c < length (k ! i ! (L ! i))"
+      using k_length(3) \<open>c \<le> m\<close> \<open>i < length k\<close> \<open>L ! i < length (k ! i)\<close> by (auto dest: nth_mem)
+    ultimately show ?thesis
+      unfolding k_i2_def k_i_def by simp
+  qed
+  have k_impl_alt_def: "k_impl (L, s) = IArray (map (\<lambda> c. Max {k_i2 i c | i. i < n_ps}) [0..<m+1])"
+    unfolding k_impl_def k_i2_def by auto
+  (* XXX more general pattern? *)
+  have Max_cong: "Max {f i | i. i < n_ps} = Max {g i | i. i < n_ps}"
+    if "\<And> i. i < n_ps \<Longrightarrow> f i = g i" for f g :: "nat \<Rightarrow> int"
+    by (rule arg_cong[where f = Max]) (force simp: that)
+  from that n_ps_gt_0 show ?thesis
+    unfolding k_impl_alt_def
+    unfolding k_i2_def[symmetric]
+    apply (clarsimp simp: k_fun_def k_i2_k cong: Max_cong)
+    apply safe
+    subgoal
+      by (subst Max_int_commute; force simp: setcompr_eq_image image_comp comp_def)
+    subgoal
+      using k_0 L_i_len[OF _ \<open>L \<in> states\<close>] by (intro linorder_class.Max_eqI) auto
+    subgoal
+      by (subst Max_int_commute; force simp: setcompr_eq_image image_comp comp_def)
+    done
+qed
+
+
+sublocale impl: Reachability_Problem_Impl
+  where trans_fun = trans_from
+  and inv_fun = inv_fun
+  and F_fun = Fi
+  and ceiling = k_impl
+  and A = prod_ta
+  and l\<^sub>0 = l\<^sub>0
+  and l\<^sub>0i = l\<^sub>0i
+  and F = "PR_CONST F"
+  and n = m
+  and k = k_fun
+  and trans_impl = trans_impl
+  and states' = states'
+  and loc_rel = loc_rel
+  apply standard
+
+(* trans_from *)
+  subgoal
+    unfolding trans_of_prod by (rule trans_from_correct)
+
+(* trans_impl *)
+  subgoal
+    apply (rule trans_from_refine)
+    done
+
+(* inv_fun *)
+  subgoal
+    unfolding trans_of_prod
+    by (rule set_mp[OF _ inv_fun_inv_of'[where R = loc_rel and S = "{(s, s'). state_rel s' s}"]])
+       (auto simp: loc_rel_def)
+
+(* state set *)
+  subgoal
+    using states'_superset by simp
+
+(* loc_rel l\<^sub>0 l\<^sub>0i*)
+  subgoal
+    using state_rel_start unfolding loc_rel_def by auto
+
+(* loc_rel left unique *)
+  subgoal for l li li'
+    unfolding trans_of_prod by (rule state_rel_left_unique)
+
+(* loc_rel right unique *)
+  subgoal for l l' li
+    unfolding trans_of_prod by (rule state_rel_right_unique)
+
+(* ceiling *)
+  subgoal
+    unfolding inv_rel_def using L\<^sub>0_states
+    by (auto simp: loc_rel_def state_rel_def reach.k'_def k_fun_def k_impl_k_fun)
+
+(* F_fun *)
+  subgoal
+    unfolding inv_rel_def by (clarsimp dest!: F_Fi)
+
+  done
+
+end (* Generalized_Network_Impl_nat_ceiling_start_state *)
+
+no_notation UPPAAL_Model_Checking.models ("_,_ \<Turnstile>\<^sub>_ _" [61,61] 61)
+
+
+context Reachability_Problem_Impl
+begin
+
+lemma F_reachable_correct:
+  "op.F_reachable
+  \<longleftrightarrow> (\<exists>l'. \<forall>u\<^sub>0. (\<forall>c \<in> {1..n}. u\<^sub>0 c = 0) \<longrightarrow> (\<exists> u'. conv_A A \<turnstile>' \<langle>l\<^sub>0, u\<^sub>0\<rangle> \<rightarrow>* \<langle>l', u'\<rangle> \<and> F l'))"
+  using E_op''.E_from_op_reachability_check[symmetric] reachability_check_new
+  unfolding E_op_F_reachable E_op''.F_reachable_def E_op''.reachable_def
+  unfolding F_rel_def by auto
+
+lemma E_op''_F_reachable_correct:
+  "E_op''.F_reachable
+  \<longleftrightarrow> (\<exists>l'. \<forall>u\<^sub>0. (\<forall>c \<in> {1..n}. u\<^sub>0 c = 0) \<longrightarrow> (\<exists> u'. conv_A A \<turnstile>' \<langle>l\<^sub>0, u\<^sub>0\<rangle> \<rightarrow>* \<langle>l', u'\<rangle> \<and> F l'))"
+  using E_op''.E_from_op_reachability_check[symmetric] reachability_check_new
+  unfolding E_op_F_reachable E_op''.F_reachable_def E_op''.reachable_def
+  unfolding F_rel_def by auto
+
+lemma Ex_ev_impl_hnr:
+  assumes "\<forall>u\<^sub>0. (\<forall>c \<in> {1..n}. u\<^sub>0 c = 0) \<longrightarrow> \<not> deadlock (l\<^sub>0, u\<^sub>0)"
+  shows
+    "
+  (uncurry0
+    (pw_impl (return \<circ> fst) state_copy_impl tracei subsumes_impl a\<^sub>0_impl F_impl succs_impl
+      emptiness_check_impl),
+   uncurry0 (SPEC (\<lambda>r. (r \<longleftrightarrow> (\<forall>u\<^sub>0. (\<forall>c \<in> {1..n}. u\<^sub>0 c = 0) \<longrightarrow> Ex_ev (\<lambda>(l, _). F l) (l\<^sub>0, u\<^sub>0))))))
+  \<in> unit_assn\<^sup>k \<rightarrow>\<^sub>a bool_assn"
+proof -
+  interpret Bisimulation_Invariant
+    "(\<lambda>(l, u) (l', u'). conv_A A \<turnstile>' \<langle>l, u\<rangle> \<rightarrow> \<langle>l', u'\<rangle>)"
+    "(\<lambda>(l, u) (l', u'). conv_A A \<turnstile>' \<langle>l, u\<rangle> \<rightarrow> \<langle>l', u'\<rangle>)"
+    "(\<lambda>(l, u) (l', u'). l' = l \<and> (\<forall> c. c \<in> clk_set (conv_A A) \<longrightarrow> u c = u' c))"
+    "(\<lambda>_. True)" "(\<lambda>_. True)"
+    apply (rule ta_bisimulation)
+    done
+  define spec where "spec = (\<forall>u\<^sub>0. (\<forall>c \<in> {1..n}. u\<^sub>0 c = 0) \<longrightarrow> Ex_ev (\<lambda>(l, _). F l) (l\<^sub>0, u\<^sub>0))"
+  have *: "E_op''.F_reachable \<longleftrightarrow> spec"
+    unfolding spec_def
+    unfolding E_op''_F_reachable_correct
+  proof safe
+    fix l' :: \<open>'s\<close> and u\<^sub>0 :: \<open>nat \<Rightarrow> real\<close>
+    assume
+      \<open>\<forall>u\<^sub>0. (\<forall>c\<in>{1..n}. u\<^sub>0 c = 0) \<longrightarrow> (\<exists>u'. conv_A A \<turnstile>' \<langle>l\<^sub>0, u\<^sub>0\<rangle> \<rightarrow>* \<langle>l', u'\<rangle> \<and> F l')\<close> and
+      \<open>\<forall>c\<in>{1..n}. u\<^sub>0 c = 0\<close>
+    then show \<open>Ex_ev (\<lambda>(l, _). F l) (l\<^sub>0, u\<^sub>0)\<close>
+      using assms by (subst Ex_ev; unfold reaches_steps'[symmetric]) blast+
+  next
+    assume \<open>\<forall>u\<^sub>0. (\<forall>c\<in>{1..n}. u\<^sub>0 c = 0) \<longrightarrow> Ex_ev (\<lambda>(l, _). F l) (l\<^sub>0, u\<^sub>0)\<close>
+    then have "Ex_ev (\<lambda>(l, _). F l) (l\<^sub>0, \<lambda>_. 0)"
+      by auto
+    then obtain l' u' where "conv_A A \<turnstile>' \<langle>l\<^sub>0, (\<lambda>_. 0)\<rangle> \<rightarrow>* \<langle>l', u'\<rangle> \<and> F l'"
+      apply (subst (asm) Ex_ev)
+      using assms
+      unfolding reaches_steps'[symmetric]
+      by auto
+    then show \<open>\<exists>l'. \<forall>u\<^sub>0. (\<forall>c\<in>{1..n}. u\<^sub>0 c = 0) \<longrightarrow> (\<exists>u'. conv_A A \<turnstile>' \<langle>l\<^sub>0, u\<^sub>0\<rangle> \<rightarrow>* \<langle>l', u'\<rangle> \<and> F l')\<close>
+    proof (inst_existentials l', clarsimp, unfold reaches_steps'[symmetric])
+      fix u\<^sub>0 :: \<open>nat \<Rightarrow> real\<close>
+      assume \<open>reaches (l\<^sub>0, \<lambda>_. 0) (l', u')\<close> and \<open>F l'\<close> and \<open>\<forall>c\<in>{Suc 0..n}. u\<^sub>0 c = 0\<close>
+      then have "equiv' (l\<^sub>0, \<lambda>_. 0) (l\<^sub>0, u\<^sub>0)"
+        unfolding equiv'_def using clocks_I[of "\<lambda>_. 0" u\<^sub>0] by auto
+      with \<open>reaches _ _\<close> show \<open>\<exists>u'. reaches (l\<^sub>0, u\<^sub>0) (l', u')\<close>
+        by - (drule (1) bisim.A_B.simulation_reaches, unfold equiv'_def, auto)
+    qed
+  qed
+  show ?thesis
+    unfolding spec_def[symmetric] using pw_impl_hnr_F_reachable[to_hnr, unfolded hn_refine_def]
+    by sepref_to_hoare (sep_auto simp: *)
+qed
+
+end (* Reachability Problem Impl *)
+
+
+
+
+
+
+
+
+
+
+
+context Generalized_Network_Impl_nat_urge
+begin
+
+sublocale conv: Prod_TA_urge
+  "(set syncs, map (Generalized_Network_Language.conv_A o automaton_of) automata, map_of bounds')"
+  by standard
+     (use no_urgency in \<open>auto simp: Generalized_Network_Language.conv_A_def automaton_of_def urgent_def\<close>)
+
+abbreviation "A \<equiv> (set syncs, map automaton_of automata, map_of bounds')"
+
+interpretation conv_eq_bisim:
+  Bisimulation_Invariant
+  "(\<lambda>(l, u) (l', u'). conv_A prod_ta \<turnstile>' \<langle>l, u\<rangle> \<rightarrow> \<langle>l', u'\<rangle>)"
+  "(\<lambda>(L, s, u) (L', s', u'). conv.prod_ta   \<turnstile>' \<langle>(L, s), u\<rangle> \<rightarrow> \<langle>(L', s'), u'\<rangle>)"
+  "(\<lambda>((L, s), u) (L', s', u'). L = L' \<and> u = u' \<and> s = s')"
+  "(\<lambda>((L, s), u). conv.all_prop L s)"
+  "(\<lambda>(L, s, u). conv.all_prop L s)"
+proof goal_cases
+  case 1
+  interpret Bisimulation_Invariant
+  "(\<lambda>(L, s, u) (L', s', u'). conv_A prod_ta \<turnstile>' \<langle>(L, s), u\<rangle> \<rightarrow> \<langle>(L', s'), u'\<rangle>)"
+  "(\<lambda>(L, s, u) (L', s', u'). conv.prod_ta   \<turnstile>' \<langle>(L, s), u\<rangle> \<rightarrow> \<langle>(L', s'), u'\<rangle>)"
+  "(=)"
+  "(\<lambda>(L, s, u). conv.all_prop L s)"
+  "(\<lambda>(L, s, u). conv.all_prop L s)"
+  by (rule Bisimulation_Invariant_strong_intro)
+     (auto simp: conv_prod_ta elim: conv.prod_all_prop_inv')
+  show ?case
+    by standard (auto simp: conv_prod_ta elim: conv.prod_all_prop_inv')
+qed
+
+interpretation Bisimulation_Invariant
+  "(\<lambda>(l, u) (l', u'). conv_A prod_ta \<turnstile>' \<langle>l, u\<rangle> \<rightarrow> \<langle>l', u'\<rangle>)"
+  "(\<lambda>(L, s, u) (L', s', u'). Generalized_Network_Language.conv A \<turnstile> \<langle>L, s, u\<rangle> \<rightarrow> \<langle>L', s', u'\<rangle>)"
+  "(\<lambda>((L, s), u) (L', s', u'). L = L' \<and> u = u' \<and> s = s')"
+  "(\<lambda>((L, s), u). conv.all_prop L s)"
+  "(\<lambda>(L, s, u). conv.all_prop L s)"
+  unfolding conv_alt_def
+  apply (rule Bisimulation_Invariant_sim_replace, rule Bisimulation_Invariant_composition)
+    apply (rule conv_eq_bisim.Bisimulation_Invariant_axioms conv.prod_bisim_intro)+
+  apply auto
+  done
+
+lemmas prod_bisim = Bisimulation_Invariant_axioms
+
+lemmas deadlock_iff = deadlock_iff
+
+lemma conv_all_prop:
+  "conv.all_prop = all_prop"
+  unfolding conv.all_prop_def all_prop_def by simp
+
+thm Ex_ev_iff
+thm CTL_compatible[THEN rel_funD, symmetric]
+
+definition prop_of2 where
+  "prop_of2 \<phi> = PropC (\<lambda>((L, s), _). check_sexp \<phi> L (the o s))"
+
+fun ctl_of2 where
+  "ctl_of2 (formula.EX \<phi>) = ctl_formula.EX (prop_of2 \<phi>)"
+| "ctl_of2 (formula.EG \<phi>) = ctl_formula.EG (prop_of2 \<phi>)"
+| "ctl_of2 (formula.AX \<phi>) = ctl_formula.AX (prop_of2 \<phi>)"
+| "ctl_of2 (formula.AG \<phi>) = ctl_formula.AG (prop_of2 \<phi>)"
+| "ctl_of2 (formula.Leadsto \<phi> \<psi>) =
+  ctl_formula.AG (ctl_formula.ImpliesC (prop_of2 \<phi>) (ctl_formula.AX (prop_of2 \<psi>)))"
+
+lemma models_correct:
+  "Generalized_Network_Language.conv A,(L\<^sub>0, s\<^sub>0, u\<^sub>0) \<Turnstile> \<Phi> = (case \<Phi> of
+    formula.EX \<phi> \<Rightarrow>
+      Graph_Defs.Ex_ev
+        (\<lambda> (l, u) (l', u'). conv_A prod_ta \<turnstile>' \<langle>l, u\<rangle> \<rightarrow> \<langle>l', u'\<rangle>)
+        (\<lambda> ((L, s), _). check_sexp \<phi> L (the o s))
+  | formula.EG \<phi> \<Rightarrow>
+      Not o Graph_Defs.Alw_ev
+        (\<lambda> (l, u) (l', u'). conv_A prod_ta \<turnstile>' \<langle>l, u\<rangle> \<rightarrow> \<langle>l', u'\<rangle>)
+        (\<lambda> ((L, s), _). \<not> check_sexp \<phi> L (the o s))
+  | formula.AX \<phi> \<Rightarrow>
+      Graph_Defs.Alw_ev
+        (\<lambda> (l, u) (l', u'). conv_A prod_ta \<turnstile>' \<langle>l, u\<rangle> \<rightarrow> \<langle>l', u'\<rangle>)
+        (\<lambda> ((L, s), _). check_sexp \<phi> L (the o s))
+  | formula.AG \<phi> \<Rightarrow>
+      Not o Graph_Defs.Ex_ev
+        (\<lambda> (l, u) (l', u'). conv_A prod_ta \<turnstile>' \<langle>l, u\<rangle> \<rightarrow> \<langle>l', u'\<rangle>)
+        (\<lambda> ((L, s), _). \<not> check_sexp \<phi> L (the o s))
+  | formula.Leadsto \<phi> \<psi> \<Rightarrow>
+      Graph_Defs.leadsto
+        (\<lambda> (l, u) (l', u'). conv_A prod_ta \<turnstile>' \<langle>l, u\<rangle> \<rightarrow> \<langle>l', u'\<rangle>)
+        (\<lambda> ((L, s), _). check_sexp \<phi> L (the o s))
+        (\<lambda> ((L, s), _). check_sexp \<psi> L (the o s))
+  ) ((L\<^sub>0, s\<^sub>0), u\<^sub>0)
+  " if "L\<^sub>0 \<in> states" "bounded bounds s\<^sub>0"
+proof -
+  have *: "((Not \<circ>\<circ> case_prod) (\<lambda>(L, s) _. check_sexp \<phi> L (the o s)))
+    = (\<lambda>((L, s), _). \<not> check_sexp \<phi> L (the o s))"
+    for \<phi> by (auto simp: comp_def)
+  have "rel_ctl_formula compatible (ctl_of2 \<Phi>) (ctl_of \<Phi>)"
+    by (cases \<Phi>; simp add: prop_of_def prop_of2_def rel_fun_def A_B.equiv'_def)
+  moreover have "A_B.equiv' ((L\<^sub>0, s\<^sub>0), u\<^sub>0) (L\<^sub>0, s\<^sub>0, u\<^sub>0)"
+    unfolding A_B.equiv'_def unfolding conv_all_prop all_prop_def using that by simp
+  ultimately show ?thesis
+    apply (subst models_ctl_iff)
+    apply (subst CTL_compatible[THEN rel_funD, symmetric])
+      apply assumption+
+    apply (cases \<Phi>; simp add:
+        Graph_Defs.models_ctl.simps prop_of2_def
+        Graph_Defs.Ex_alw_iff Graph_Defs.Alw_alw_iff Graph_Defs.leadsto_def *)
+    done
+qed
+
+end (* Generalized_Network_Impl_nat *)
+
+context Generalized_Network_Impl_nat_ceiling_start_state
+begin
+
+definition Alw_ev_checker where
+  "Alw_ev_checker = dfs_map_impl'
+     (impl.succs_P_impl' Fi) impl.a\<^sub>0_impl impl.subsumes_impl (return \<circ> fst)
+     impl.state_copy_impl"
+
+definition leadsto_checker where
+  "leadsto_checker \<psi> = do {
+      r \<leftarrow> leadsto_impl
+      impl.state_copy_impl (impl.succs_P_impl' (\<lambda> (L, s). \<not> check_sexpi \<psi> L s))
+      impl.a\<^sub>0_impl impl.subsumes_impl (return \<circ> fst)
+      impl.succs_impl' impl.emptiness_check_impl impl.F_impl
+      (impl.Q_impl (\<lambda> (L, s). \<not> check_sexpi \<psi> L s))
+      impl.tracei;
+      return (\<not> r)
+    }"
+
+definition
+  "reachability_checker \<equiv>
+     pw_impl
+      (return o fst) impl.state_copy_impl impl.tracei impl.subsumes_impl impl.a\<^sub>0_impl impl.F_impl
+      impl.succs_impl impl.emptiness_check_impl"
+
+definition model_checker where
+  "model_checker = (
+  case formula of
+    formula.EX _ \<Rightarrow> reachability_checker |
+    formula.AG _ \<Rightarrow> do {
+      r \<leftarrow> reachability_checker;
+      return (\<not> r)
+    } |
+    formula.AX _ \<Rightarrow> do {
+      r \<leftarrow> if PR_CONST F l\<^sub>0
+      then Alw_ev_checker
+      else return False;
+      return (\<not> r)
+    } |
+    formula.EG _ \<Rightarrow>
+      if PR_CONST F l\<^sub>0
+      then Alw_ev_checker
+      else return False |
+    formula.Leadsto _ \<psi> \<Rightarrow> leadsto_checker \<psi>
+  )
+  "
+
+abbreviation "u\<^sub>0 \<equiv> (\<lambda> _. 0 :: real)"
+
+lemma all_prop_start:
+  "all_prop L\<^sub>0 (map_of s\<^sub>0)"
+  using L\<^sub>0_states s\<^sub>0_bounded unfolding all_prop_def ..
+
+lemma deadlock_start_iff:
+  "Graph_Defs.deadlock
+   (\<lambda>(L, s, u) (L', s', u'). Generalized_Network_Language.conv A \<turnstile> \<langle>L, s, u\<rangle> \<rightarrow> \<langle>L', s', u'\<rangle>) (L\<^sub>0, (map_of s\<^sub>0), u\<^sub>0)
+  \<longleftrightarrow> reach.deadlock (l\<^sub>0, u\<^sub>0)"
+  using all_prop_start by (subst deadlock_iff[symmetric]) (auto simp: conv_all_prop)
+
+lemma F_Fi':
+  "check_sexp \<psi> L (the o s) \<longleftrightarrow> check_sexpi \<psi> L' s'"
+  if "((L', s'), (L, s)) \<in> loc_rel" "formula = Leadsto \<phi> \<psi>"
+  using vars_of_formula that unfolding loc_rel_def by (auto elim!: check_sexp_check_sexpi)
+
+theorem model_check':
+  "(uncurry0 model_checker,
+    uncurry0 (
+      SPEC (\<lambda>r.
+  \<not> Graph_Defs.deadlock
+    (\<lambda>(L, s, u) (L', s', u').
+      Generalized_Network_Language.conv A \<turnstile> \<langle>L, s, u\<rangle> \<rightarrow> \<langle>L', s', u'\<rangle>) (L\<^sub>0, (map_of s\<^sub>0), u\<^sub>0)
+      \<longrightarrow> r = (Generalized_Network_Language.conv A,(L\<^sub>0, (map_of s\<^sub>0), u\<^sub>0) \<Turnstile> formula)
+      )
+    )
+   )
+  \<in> unit_assn\<^sup>k \<rightarrow>\<^sub>a bool_assn"
+proof -
+  define protect where
+    "protect = ((\<lambda>(l, u) (l', u'). conv_A prod_ta \<turnstile>' \<langle>l, u\<rangle> \<rightarrow> \<langle>l', u'\<rangle>))"
+
+  have start: "l\<^sub>0 \<in> Normalized_Zone_Semantics_Impl_Refine.state_set trans_prod"
+    if "\<not> Graph_Defs.deadlock protect (l\<^sub>0, \<lambda>_. 0)"
+    using that unfolding protect_def by (rule impl.init_state_in_state_set[simplified])
+
+  interpret ta_bisim: Bisimulation_Invariant
+    "(\<lambda>(l, u) (l', u'). conv_A prod_ta \<turnstile>' \<langle>l, u\<rangle> \<rightarrow> \<langle>l', u'\<rangle>)"
+    "(\<lambda>(l, u) (l', u'). conv_A prod_ta \<turnstile>' \<langle>l, u\<rangle> \<rightarrow> \<langle>l', u'\<rangle>)"
+    "(\<lambda>(l, u) (l', u'). l' = l \<and> (\<forall> c. c \<in> clk_set (conv_A prod_ta) \<longrightarrow> u c = u' c))"
+    "(\<lambda>_. True)" "(\<lambda>_. True)"
+    by (rule ta_bisimulation[of "conv_A prod_ta"])
+
+  let ?\<phi>1 = "\<lambda>\<phi>. \<lambda>(p, _). case p of (L, s) \<Rightarrow> \<not> check_sexp \<phi> L (the \<circ> s)"
+  let ?\<phi>2 = "\<lambda>\<phi>. \<lambda>(p, _). case p of (L, s) \<Rightarrow> check_sexp \<phi> L (the \<circ> s)"
+
+  have start_sim:
+    "ta_bisim.A_B.equiv' (l\<^sub>0, u) (l\<^sub>0, \<lambda>_. 0)" "ta_bisim.A_B.equiv' (l\<^sub>0, \<lambda>_. 0) (l\<^sub>0, u)"
+    if "\<forall>c\<in>{Suc 0..m}. u c = 0" for u
+    using impl.clocks_I[of u "\<lambda>_. 0"] that unfolding ta_bisim.A_B.equiv'_def by auto
+
+  have compatibleI: "\<phi> a = \<phi> b"
+    if "ta_bisim.A_B.equiv' a b" "\<And> l u u'. \<phi> (l, u) = \<phi> (l, u')" for a b \<phi>
+    using that unfolding ta_bisim.A_B.equiv'_def by auto
+
+  have bisims:
+    "(\<forall>u\<^sub>0. (\<forall>c\<in>{Suc 0..m}. u\<^sub>0 c = 0) \<longrightarrow> reach.Ex_ev (?\<phi>1 \<phi>) (l\<^sub>0, u\<^sub>0))
+    \<longleftrightarrow> reach.Ex_ev (?\<phi>1 \<phi>) (l\<^sub>0, u\<^sub>0)"
+    "(\<forall>u\<^sub>0. (\<forall>c\<in>{Suc 0..m}. u\<^sub>0 c = 0) \<longrightarrow> reach.Ex_ev (?\<phi>2 \<phi>) (l\<^sub>0, u\<^sub>0))
+    \<longleftrightarrow> reach.Ex_ev (?\<phi>2 \<phi>) (l\<^sub>0, u\<^sub>0)"
+    "(\<forall>u\<^sub>0. (\<forall>c\<in>{Suc 0..m}. u\<^sub>0 c = 0) \<longrightarrow> reach.Alw_ev (?\<phi>1 \<phi>) (l\<^sub>0, u\<^sub>0))
+    \<longleftrightarrow> reach.Alw_ev (?\<phi>1 \<phi>) (l\<^sub>0, u\<^sub>0)"
+    "(\<forall>u\<^sub>0. (\<forall>c\<in>{Suc 0..m}. u\<^sub>0 c = 0) \<longrightarrow> reach.Alw_ev (?\<phi>2 \<phi>) (l\<^sub>0, u\<^sub>0))
+    \<longleftrightarrow> reach.Alw_ev (?\<phi>2 \<phi>) (l\<^sub>0, u\<^sub>0)"
+    "(\<forall>u\<^sub>0. (\<forall>c\<in>{Suc 0..m}. u\<^sub>0 c = 0) \<longrightarrow> reach.leadsto (?\<phi>2 \<phi>) (?\<phi>2 \<psi>) (l\<^sub>0, u\<^sub>0))
+    \<longleftrightarrow> reach.leadsto (?\<phi>2 \<phi>) (?\<phi>2 \<psi>) (l\<^sub>0, u\<^sub>0)"
+    for \<phi> \<psi>
+        apply auto
+    subgoal for u
+      using start_sim
+      by (subst (asm) ta_bisim.Ex_ev_iff[of "?\<phi>1 \<phi>" "?\<phi>1 \<phi>"]) (erule compatibleI, auto)
+    subgoal for u
+      using start_sim
+      by (subst (asm) ta_bisim.Ex_ev_iff[of "?\<phi>2 \<phi>" "?\<phi>2 \<phi>"]) (erule compatibleI, auto)
+    subgoal for u
+      using start_sim
+      by (subst (asm) ta_bisim.Alw_ev_iff[of "?\<phi>1 \<phi>" "?\<phi>1 \<phi>"]) (erule compatibleI, auto)
+    subgoal for u
+      using start_sim
+      by (subst (asm) ta_bisim.Alw_ev_iff[of "?\<phi>2 \<phi>" "?\<phi>2 \<phi>"]) (erule compatibleI, auto)
+    subgoal for u
+      using start_sim
+      by (subst (asm) ta_bisim.Leadsto_iff[of "?\<phi>2 \<phi>" "?\<phi>2 \<phi>" "?\<phi>2 \<psi>" "?\<phi>2 \<psi>"])
+        ((erule compatibleI)?; auto)+
+    done
+
+  have deadlock_bisim:
+    "(\<forall>u\<^sub>0. (\<forall>c\<in>{1..m}. u\<^sub>0 c = 0) \<longrightarrow> \<not> reach.deadlock (l\<^sub>0, u\<^sub>0))
+    \<longleftrightarrow> \<not> Graph_Defs.deadlock protect (l\<^sub>0, \<lambda>_. 0)"
+    unfolding protect_def
+    apply (safe; clarsimp)
+    apply (drule start_sim(2))
+    apply (subst (asm) ta_bisim.deadlock_iff)
+    unfolding ta_bisim.A_B.equiv'_def
+    by auto
+
+  have *****:
+    "return True = (return False \<bind> return o Not)"
+    by auto
+
+  show ?thesis
+    unfolding deadlock_start_iff
+    using models_correct[OF L\<^sub>0_states s\<^sub>0_bounded]
+    unfolding protect_def[symmetric]
+    apply (simp split del: if_split)
+    apply sepref_to_hoare
+    apply sep_auto
+    unfolding model_checker_def Alw_ev_checker_def leadsto_checker_def reachability_checker_def
+    apply (cases formula; simp)
+
+    subgoal
+      apply (cases "Graph_Defs.deadlock protect (l\<^sub>0, \<lambda>_. 0)")
+      subgoal
+        using impl.pw_impl_hnr_F_reachable[to_hnr, unfolded hn_refine_def]
+        by (sep_auto elim!: cons_post_rule)
+      subgoal
+        using impl.Ex_ev_impl_hnr[unfolded deadlock_bisim, to_hnr, unfolded hn_refine_def]
+        by (sep_auto simp: pure_def protect_def bisims)
+      done
+
+    subgoal premises prems for \<phi>
+    proof -
+      have *: "(\<lambda>(l, u). \<not> F l) = ((\<lambda>(p, _). case p of (L, s) \<Rightarrow> \<not> check_sexp \<phi> L (the \<circ> s)))"
+        using prems by auto
+      show ?thesis
+        using impl.Alw_ev_impl_hnr[to_hnr, unfolded hn_refine_def] prems start
+        unfolding PR_CONST_def * protect_def
+        by (sep_auto elim!: cons_post_rule simp: pure_def bisims)
+    qed
+
+    subgoal premises prems for \<phi>
+    proof -
+      have *: "(\<lambda>(l, u). \<not> F l) = ((\<lambda>(p, _). case p of (L, s) \<Rightarrow> check_sexp \<phi> L (the \<circ> s)))"
+        using prems by auto
+      show ?thesis
+        apply intros
+        subgoal
+          using impl.Alw_ev_impl_hnr[to_hnr, unfolded hn_refine_def] prems start
+          unfolding PR_CONST_def * protect_def
+          apply simp
+          unfolding *****
+          apply (erule bind_rule)
+          apply (sep_auto simp: pure_def bisims(2-))
+          done
+        subgoal
+          using impl.Alw_ev_impl_hnr[to_hnr, unfolded hn_refine_def] prems start
+          unfolding PR_CONST_def * protect_def
+          apply (sep_auto elim!: cons_post_rule simp: pure_def bisims(2-))
+          done
+        done
+    qed
+
+    subgoal
+      apply (cases "Graph_Defs.deadlock protect (l\<^sub>0, \<lambda>_. 0)")
+      subgoal
+        using impl.pw_impl_hnr_F_reachable[to_hnr, unfolded hn_refine_def]
+        by (sep_auto elim!: cons_post_rule)
+      subgoal
+        using impl.Ex_ev_impl_hnr[unfolded deadlock_bisim, to_hnr, unfolded hn_refine_def]
+        apply (sep_auto simp: pure_def protect_def bisims)
+        done
+      done
+
+    subgoal premises prems for \<phi> \<psi>
+    proof -
+      have *: "(\<lambda>(l, u). F l) = ((\<lambda>(p, _). case p of (L, s) \<Rightarrow> check_sexp \<phi> L (the \<circ> s)))"
+        using prems by auto
+      have **:"(\<lambda>(L, s). \<not> check_sexpi \<psi> L s, \<lambda>(L, s). \<not> check_sexp \<psi> L (the \<circ> s))
+               \<in> inv_rel loc_rel states'"
+        unfolding trans_of_prod using prems by (auto simp: F_Fi' inv_rel_def)
+      have ****: "(\<lambda>(l, u). \<not> (case l of (L, s) \<Rightarrow> \<not> check_sexp \<psi> L (the \<circ> s)))
+      = (\<lambda>(l, u). (case l of (L, s) \<Rightarrow> check_sexp \<psi> L (the \<circ> s)))"
+        by auto
+      show ?thesis
+        apply (cases "reach.deadlock (l\<^sub>0, \<lambda>_. 0)")
+        subgoal
+          using impl.leadsto_impl_hnr'[OF **, to_hnr, unfolded hn_refine_def]
+          unfolding protect_def \<open>formula = _\<close> by (sep_auto simp: pure_def)
+        using impl.leadsto_impl_hnr[unfolded deadlock_bisim, to_hnr, unfolded hn_refine_def, OF **]
+          prems start
+        unfolding PR_CONST_def * protect_def by (sep_auto simp: pure_def bisims ****)
+    qed
+    done
+qed
+
+
+subsection \<open>Extracting an efficient implementation\<close>
+
+lemma reachability_checker_alt_def':
+  "reachability_checker \<equiv>
+    do {
+      x \<leftarrow> do {
+        let key = return \<circ> fst;
+        let sub = impl.subsumes_impl;
+        let copy = impl.state_copy_impl;
+        let start = impl.a\<^sub>0_impl;
+        let final = impl.F_impl;
+        let succs =  impl.succs_impl;
+        let empty = impl.emptiness_check_impl;
+        let trace = impl.tracei;
+        pw_impl key copy trace sub start final succs empty
+      };
+      _ \<leftarrow> return ();
+      return x
+    }"
+  unfolding reachability_checker_def by simp
+
+lemma Alw_ev_checker_alt_def':
+  "Alw_ev_checker \<equiv>
+    do {
+      x \<leftarrow> let
+        key = return \<circ> fst;
+        sub = impl.subsumes_impl;
+        copy = impl.state_copy_impl;
+        start = impl.a\<^sub>0_impl;
+        succs =  impl.succs_P_impl' Fi
+      in dfs_map_impl' succs start sub key copy;
+      _ \<leftarrow> return ();
+      return x
+    }"
+  unfolding Alw_ev_checker_def by simp
+
+lemma leadsto_checker_alt_def':
+  "leadsto_checker \<psi> \<equiv>
+    do {
+      r \<leftarrow> let
+        key = return \<circ> fst;
+        sub = impl.subsumes_impl;
+        copy = impl.state_copy_impl;
+        start = impl.a\<^sub>0_impl;
+        final = impl.F_impl;
+        final' = (impl.Q_impl (\<lambda>(L, s). \<not> check_sexpi \<psi> L s));
+        succs =  impl.succs_P_impl' (\<lambda>(L, s). \<not> check_sexpi \<psi> L s);
+        succs' =  impl.succs_impl';
+        empty = impl.emptiness_check_impl;
+        trace = impl.tracei
+      in
+        leadsto_impl copy succs start sub key succs' empty final final' trace;
+      return (\<not> r)
+    }"
+  unfolding leadsto_checker_def by simp
+
+theorem k_impl_alt_def:
+  "k_impl = (\<lambda>(l, s). IArray (map (\<lambda>c. MAX i \<in> {0..<n_ps}. k_i !! i !! (l ! i) !! c) [0..<m + 1]))"
+proof -
+  have "{i. i < p} = {0..<p}" for p :: nat
+    by auto
+  then show ?thesis
+    unfolding k_impl_def setcompr_eq_image by simp
+qed
+
+definition
+  "trans_map_inner \<equiv> map (\<lambda>i. union_map_of (fst (snd (snd (automata ! i))))) [0..<n_ps]"
+
+lemma trans_map_alt_def:
+  "trans_map i j = (case (IArray trans_map_inner !! i) j of None \<Rightarrow> [] | Some xs \<Rightarrow> xs)"
+  if "i < n_ps"
+  using that unfolding trans_map_inner_def trans_map_def by (auto simp: n_ps_def)
+
+schematic_goal succs_impl_alt_def:
+  "impl.succs_impl \<equiv> ?impl"
+  unfolding impl.succs_impl_def
+  apply (abstract_let impl.E_op''_impl E_op''_impl)
+  unfolding impl.E_op''_impl_def fw_impl'_int
+  apply (abstract_let trans_impl trans_impl)
+  unfolding trans_impl_def
+  apply (abstract_let int_trans_impl int_trans_impl)
+  apply (abstract_let sync_trans_from_impl sync_trans_impl)
+  unfolding int_trans_impl_def sync_trans_from_impl_def
+  apply (abstract_let trans_com_grouped trans_com_grouped)
+  apply (abstract_let int_trans_from_all_impl int_trans_from_all_impl)
+  unfolding int_trans_from_all_impl_def
+  apply (abstract_let int_trans_from_vec_impl int_trans_from_vec_impl)
+  unfolding int_trans_from_vec_impl_def
+  apply (abstract_let int_trans_from_loc_impl int_trans_from_loc_impl)
+  unfolding int_trans_from_loc_impl_def
+  apply (abstract_let trans_i_map trans_i_map)
+  unfolding trans_com_grouped_def
+  unfolding trans_i_map_def
+  apply (abstract_let trans_map trans_map)
+  apply (abstract_let "inv_fun :: nat list \<times> int list \<Rightarrow> _" inv_fun)
+  unfolding inv_fun_alt_def
+  apply (abstract_let invs2 invs)
+  unfolding invs2_def
+  unfolding k_impl_alt_def
+  apply (abstract_let k_i k_i) (* Could be killed *)
+  apply (abstract_let n_ps n_ps)
+  by (rule Pure.reflexive)
+
+schematic_goal succs_P_impl_alt_def:
+  "impl.succs_P_impl Pi \<equiv> ?impl"
+  if "(Pi, P) \<in> inv_rel loc_rel states'"
+  for P Pi
+  unfolding impl.succs_P_impl_def[OF that]
+  apply (abstract_let impl.E_op''_impl E_op''_impl)
+  unfolding impl.E_op''_impl_def fw_impl'_int
+  apply (abstract_let "trans_impl" trans_impl)
+  unfolding trans_impl_def
+  apply (abstract_let "int_trans_impl" int_trans_impl)
+  apply (abstract_let "sync_trans_from_impl" sync_trans_impl)
+  unfolding int_trans_impl_def sync_trans_from_impl_def
+  apply (abstract_let trans_com_grouped trans_com_grouped)
+  apply (abstract_let int_trans_from_all_impl int_trans_from_all_impl)
+  unfolding int_trans_from_all_impl_def
+  apply (abstract_let int_trans_from_vec_impl int_trans_from_vec_impl)
+  unfolding int_trans_from_vec_impl_def
+  apply (abstract_let int_trans_from_loc_impl int_trans_from_loc_impl)
+  unfolding int_trans_from_loc_impl_def
+  apply (abstract_let trans_i_map trans_i_map)
+  unfolding trans_com_grouped_def
+  unfolding trans_i_map_def
+  apply (abstract_let trans_map trans_map)
+  apply (abstract_let "inv_fun :: nat list \<times> int list \<Rightarrow> _" inv_fun)
+  unfolding inv_fun_alt_def
+  apply (abstract_let invs2 invs)
+  unfolding invs2_def
+  unfolding k_impl_alt_def
+  apply (abstract_let k_i k_i) (* Could be killed *)
+  apply (abstract_let n_ps n_ps)
+  by (rule Pure.reflexive)
+
+
+(* XXX These implementations contain unnecessary list reversals *)
+lemmas succs_P'_impl_alt_def =
+  impl.succs_P_impl'_def[OF impl.F_fun, unfolded succs_P_impl_alt_def[OF impl.F_fun]]
+
+schematic_goal Alw_ev_checker_alt_def:
+  "Alw_ev_checker \<equiv> ?impl"
+  unfolding Alw_ev_checker_alt_def'
+  unfolding succs_P'_impl_alt_def
+  unfolding k_impl_alt_def k_i_def
+  (* The following are just to unfold things that should have been defined in a defs locale *)
+  unfolding impl.E_op''_impl_def impl.abstr_repair_impl_def impl.abstra_repair_impl_def
+  unfolding
+    impl.start_inv_check_impl_def impl.unbounded_dbm_impl_def
+    impl.unbounded_dbm'_def
+  unfolding impl.init_dbm_impl_def impl.a\<^sub>0_impl_def
+  unfolding impl.F_impl_def
+  unfolding impl.subsumes_impl_def
+  unfolding impl.emptiness_check_impl_def
+  unfolding impl.state_copy_impl_def
+  by (rule Pure.reflexive)
+
+lemma \<psi>_compatibleI:
+  "(\<lambda>(L, s). \<not> check_sexpi \<psi> L s, \<lambda>(L, s). \<not> check_sexp \<psi> L (the \<circ> s)) \<in> inv_rel loc_rel states'"
+  if "formula = Leadsto \<phi> \<psi>"
+  using F_Fi'[OF _ that] unfolding inv_rel_def by auto
+
+lemma Q_impl_alt_def:
+  "impl.Q_impl (\<lambda>(L, s). \<not> check_sexpi \<psi> L s) \<equiv>
+  \<lambda>xi. return (case xi of (a1, a2) \<Rightarrow> (\<lambda>(L, s). \<not> check_sexpi \<psi> L s) a1)"
+  if "formula = Leadsto \<phi> \<psi>"
+  by (intro impl.Q_impl_def[where Q = "\<lambda>(L, s). \<not> check_sexp \<psi> L (the o s)"] \<psi>_compatibleI[OF that])
+
+schematic_goal leadsto_checker_alt_def:
+  "leadsto_checker \<psi> \<equiv> ?impl" if "formula = Leadsto \<phi> \<psi>"
+  unfolding leadsto_checker_alt_def'
+  unfolding Q_impl_alt_def[OF that] impl.F_impl_def
+  unfolding impl.succs_P_impl'_def[OF \<psi>_compatibleI[OF that]]
+  unfolding succs_P_impl_alt_def[OF \<psi>_compatibleI[OF that]]
+  unfolding impl.succs_impl'_def succs_impl_alt_def
+  unfolding k_impl_alt_def k_i_def
+  (* The following are just to unfold things that should have been defined in a defs locale *)
+  unfolding impl.E_op''_impl_def impl.abstr_repair_impl_def impl.abstra_repair_impl_def
+  unfolding
+    impl.start_inv_check_impl_def impl.unbounded_dbm_impl_def
+    impl.unbounded_dbm'_def
+  unfolding impl.init_dbm_impl_def impl.a\<^sub>0_impl_def
+  unfolding impl.F_impl_def
+  unfolding impl.subsumes_impl_def
+  unfolding impl.emptiness_check_impl_def
+  unfolding impl.state_copy_impl_def
+  by (rule Pure.reflexive)
+
+schematic_goal reachability_checker_alt_def:
+  "reachability_checker \<equiv> ?impl"
+  unfolding reachability_checker_alt_def'
+  unfolding succs_impl_alt_def
+  unfolding k_impl_alt_def k_i_def
+  (* The following are just to unfold things that should have been defined in a defs locale *)
+  unfolding impl.E_op''_impl_def impl.abstr_repair_impl_def impl.abstra_repair_impl_def
+  unfolding
+    impl.start_inv_check_impl_def impl.unbounded_dbm_impl_def
+    impl.unbounded_dbm'_def
+  unfolding impl.init_dbm_impl_def impl.a\<^sub>0_impl_def
+  unfolding impl.F_impl_def
+  unfolding impl.subsumes_impl_def
+  unfolding impl.emptiness_check_impl_def
+  unfolding impl.state_copy_impl_def
+  by (rule Pure.reflexive)
+
+end (* Generalized_Network_Impl_nat_ceiling_start_state *)
+
+concrete_definition reachability_checker
+  uses Generalized_Network_Impl_nat_ceiling_start_state.reachability_checker_alt_def
+
+concrete_definition Alw_ev_checker
+  uses Generalized_Network_Impl_nat_ceiling_start_state.Alw_ev_checker_alt_def
+
+concrete_definition leadsto_checker
+  uses Generalized_Network_Impl_nat_ceiling_start_state.leadsto_checker_alt_def
+
+context Generalized_Network_Impl_nat_ceiling_start_state
+begin
+
+lemma model_checker_unfold_leadsto:
+  "model_checker = (
+  case formula of Generalized_Network_Language_Model_Checking.formula.EX xa \<Rightarrow> reachability_checker
+    | Generalized_Network_Language_Model_Checking.formula.EG xa \<Rightarrow>
+      if PR_CONST F l\<^sub>0 then Alw_ev_checker else return False
+    | Generalized_Network_Language_Model_Checking.formula.AX xa \<Rightarrow>
+      (if PR_CONST F l\<^sub>0 then Alw_ev_checker else return False) \<bind> (\<lambda>r. return (\<not> r))
+    | Generalized_Network_Language_Model_Checking.formula.AG xa \<Rightarrow>
+      reachability_checker \<bind> (\<lambda>r. return (\<not> r))
+    | Generalized_Network_Language_Model_Checking.formula.Leadsto \<phi> \<psi> \<Rightarrow>
+      Generalized_Network_Language_Model_Checking.leadsto_checker
+        syncs bounds' automata m num_states num_actions k L\<^sub>0 s\<^sub>0 formula \<psi> show_clock show_state)
+"
+  unfolding model_checker_def
+  using leadsto_checker.refine[OF Generalized_Network_Impl_nat_ceiling_start_state_axioms]
+  by (simp split: formula.split)
+
+lemmas model_checker_def_refined = model_checker_unfold_leadsto[unfolded
+    reachability_checker.refine[OF Generalized_Network_Impl_nat_ceiling_start_state_axioms]
+    Alw_ev_checker.refine[OF Generalized_Network_Impl_nat_ceiling_start_state_axioms]
+  ]
+
+end (* Generalized_Network_Impl_nat_ceiling_start_state *)
+
+concrete_definition model_checker uses
+  Generalized_Network_Impl_nat_ceiling_start_state.model_checker_def_refined
+
+definition precond_mc where
+  "precond_mc
+    show_clock show_state broadcast bounds' automata m num_states num_actions k L\<^sub>0 s\<^sub>0 formula \<equiv>
+    if Generalized_Network_Impl_nat_ceiling_start_state
+      broadcast bounds' automata m num_states num_actions k L\<^sub>0 s\<^sub>0 formula
+    then
+      model_checker
+        broadcast bounds' automata m num_states num_actions k L\<^sub>0 s\<^sub>0 formula show_clock show_state
+      \<bind> (\<lambda> x. return (Some x))
+    else return None"
+
+
+abbreviation N where
+  "N broadcast automata bounds \<equiv>
+  Generalized_Network_Language.conv
+    (set broadcast, map automaton_of automata, map_of bounds)"
+
+definition has_deadlock where
+  "has_deadlock A a\<^sub>0 \<equiv>
+    Graph_Defs.deadlock (\<lambda> (L, s, u) (L', s', u'). A \<turnstile> \<langle>L, s, u\<rangle> \<rightarrow> \<langle>L', s', u'\<rangle>) a\<^sub>0"
+
+theorem model_check:
+  "<emp> precond_mc
+    show_clock show_state syncs bounds automata m num_states num_actions k L\<^sub>0 s\<^sub>0 formula
+    <\<lambda> Some r \<Rightarrow> \<up>(
+        Generalized_Network_Impl_nat_ceiling_start_state
+          syncs bounds automata m num_states num_actions k L\<^sub>0 s\<^sub>0 formula \<and>
+        (\<not> has_deadlock (N syncs automata bounds) (L\<^sub>0, map_of s\<^sub>0, \<lambda>_ . 0) \<longrightarrow>
+          r = N syncs automata bounds,(L\<^sub>0, map_of s\<^sub>0, \<lambda>_ . 0) \<Turnstile> formula
+        ))
+     | None \<Rightarrow> \<up>(\<not> Generalized_Network_Impl_nat_ceiling_start_state
+        syncs bounds automata m num_states num_actions k L\<^sub>0 s\<^sub>0 formula)
+    >\<^sub>t"
+proof -
+  define A where "A \<equiv> N syncs automata bounds"
+  define check where "check \<equiv> A,(L\<^sub>0, map_of s\<^sub>0, \<lambda>_ . 0) \<Turnstile> formula"
+  note [sep_heap_rules] =
+    Generalized_Network_Impl_nat_ceiling_start_state.model_check'[
+      to_hnr, unfolded hn_refine_def,
+      of syncs bounds automata m num_states num_actions k L\<^sub>0 s\<^sub>0 formula,
+      unfolded UPPAAL_Reachability_Problem_precompiled_defs.init_def,
+      folded A_def check_def has_deadlock_def,
+      simplified
+      ]
+  show ?thesis
+    unfolding A_def[symmetric] check_def[symmetric]
+    unfolding precond_mc_def
+    by (sep_auto simp: model_checker.refine[symmetric] pure_def)
+qed
+
+end (* Theory *)
